Executions.v
@@ -1,5 +1,6 @@
 From hahn Require Import Hahn.
-From RelAcqProof Require Import Events.  
+From RelAcqProof Require Import Events.
+Require Import Arith. 
 Set Implicit Arguments.
 
 Record Execution {Label : Type} `{LabelProof: LabelClass Label} := {
@@ -54,7 +55,9 @@ Definition uid_unique {Label: Type} {LabelProof: LabelClass Label} (exec : Execu
 Definition well_formed_po {Label: Type} {LabelProof: LabelClass Label} (exec:Execution): Prop :=
     (forall e1 e2, po exec e1 e2 -> events exec e1 /\ events exec e2) 
     /\ 
-    forall (e:Event), (events exec) e <-> exists (e0:Event), ((events exec) e0) /\ ((po exec) e e0 \/ (po exec) e0 e). 
+    (forall (e:Event), (events exec) e <-> exists (e0:Event), ((events exec) e0) /\ ((po exec) e e0 \/ (po exec) e0 e))
+    /\ 
+    (forall e1 e2, po exec e1 e2 <-> seq_before e1 e2).  
 
 (* Expresses that an mo relation can only exist between two independent writes on the same location. *)
 Definition well_formed_mo {Label: Type} {LabelProof: LabelClass Label} (exec:Execution): Prop := 
@@ -98,4 +101,40 @@ Definition behaviour {Label: Type} {LabelProof: LabelClass Label} (X : Execution
       is_w (event_label e) /\
       lab_loc (event_label e) = l /\
       lab_val (event_label e) = v /\
-      ~(exists (e': Event), (X.(mo) e e')). 
+      ~(exists (e': Event), (X.(mo) e e')).
+
+Lemma fr_same_thread_implies_po:
+    forall {Label: Type} {LabelProof : LabelClass Label} (exec: @Execution Label LabelProof)
+           (x y : @Event Label LabelProof),
+    uid_unique exec ->
+    well_formed_po exec ->
+    well_formed_mo exec ->
+    well_formed_rf exec ->
+    fr exec x y ->
+    same_thread x y ->
+    po exec x y \/ po exec y x.
+Proof with eauto.
+    intros Label LabelProof exec x y Huniq Hwf_po Hwf_mo Hwf_rf Hfr Hst.
+    unfold well_formed_po in *. 
+    destruct Hwf_po as [Hpo_events [Hpo_connected Hpo_seq]]. 
+    destruct x as [uid1 lab1 | uid1 tid1 lab1 ];
+    destruct y as [uid2 lab2 | uid2 tid2 lab2 ]; 
+    simpl in Hst; try contradiction. 
+    destruct (lt_eq_lt_dec uid1 uid2) as [[Hlt | Heq] | Hgt]. 
+    - left. apply Hpo_seq. simpl...
+    - subst. exfalso.
+      unfold fr in Hfr.
+      destruct Hfr as [w [Hrf Hmo]].
+      unfold transp in *. 
+      destruct (Hwf_rf w (EventThread uid2 tid2 lab1) Hrf) as [_ [Hevr _]].
+      destruct (Hwf_mo w (EventThread uid2 tid2 lab2) Hmo) as [_ [Hevw _]].
+      assert (Heq : EventThread uid2 tid2 lab1 = EventThread uid2 tid2 lab2).
+      { apply Huniq... }
+      inversion Heq; subst. 
+      destruct (Hwf_mo w (EventThread uid2 tid2 lab2) Hmo) as [_ [_ [_ [_ Hneq]]]].
+      destruct (Hwf_rf w (EventThread uid2 tid2 lab2) Hrf) as [Hevw' [_ [Hiw [Hir _]]]].
+      destruct (Hwf_mo w (EventThread uid2 tid2 lab2) Hmo) as [_ [_ [Hbw _]]].
+      unfold both_write in Hbw. destruct Hbw as [_ Hiw2].
+      simpl in Hir, Hiw2. exact (is_w_not_is_r _ Hiw2 Hir).    
+    - right. apply Hpo_seq. simpl...
+Qed. 
