Arm.v
@@ -1,5 +1,6 @@
 From RelAcqProof Require Import Events. 
 From RelAcqProof Require Import Executions. 
+Require Import Arith.
 From hahn Require Import Hahn.
 
 Inductive LabelArm := 
@@ -32,14 +33,25 @@ Instance LabelClassArm: LabelClass LabelArm := {
                 | R_Acq_Pc _ _ => False
                 | R_Acq _ _    => False 
                 end;
-}.
+
+    is_w_not_is_r l := match l with
+                       | W_Rel _ _    => fun _ H => H
+                       | R_Acq_Pc _ _ => fun H _ => H
+                       | R_Acq _ _    => fun H _ => H
+                       end;
+
+    is_r_not_is_w l := match l with
+                       | W_Rel _ _    => fun H _ => H
+                       | R_Acq_Pc _ _ => fun _ H => H
+                       | R_Acq _ _    => fun _ H => H
+                       end;
+}. 
 
 Definition is_ra l := match l with 
                         | W_Rel _ _    => False 
                         | R_Acq_Pc _ _ => False 
                         | R_Acq _ _    => True
-                      end. 
-
+                      end.
 
 (* ARM axiom *)
 (* bob = ((R_acq_pc ; po) ∪ (po ; W_rel)) *)
@@ -77,4 +89,39 @@ Definition ordered_before_axiom_arm (exec: Execution): Prop :=
     irreflexive (ob exec).
 
 Definition arm_consistent (exec: Execution): Prop := 
-    well_formed exec /\ (amo exec) ≡ (rmw exec) /\ atomicity_axiom exec /\ coherence_axiom exec /\ ordered_before_axiom_arm exec. 
+    well_formed exec /\ (amo exec) ≡ (rmw exec) /\ atomicity_axiom exec /\ coherence_axiom exec /\ ordered_before_axiom_arm exec.
+
+Lemma same_thread_dec_arm:
+    forall (e1 e2 : @Event LabelArm LabelClassArm),
+    {same_thread e1 e2} + {~ same_thread e1 e2}.
+Proof with eauto.
+    intros e1 e2.
+    destruct e1; destruct e2; simpl.
+    - right...
+    - right...
+    - right...
+    - destruct (Nat.eq_dec tid tid0).
+      + left...
+      + right...
+Qed.
+
+Lemma arm_consistent_amo_is_rmw: 
+    forall (execArm: @Execution LabelArm LabelClassArm) (e0 e1: @Event LabelArm LabelClassArm),
+        (amo execArm) ≡ (rmw execArm) -> (rmw execArm) e0 e1 -> (amo execArm) e0 e1.
+Proof with eauto. 
+    intros.
+    unfold same_relation in *. destruct H as [Hamo Hrmw]. 
+    unfold inclusion in *...      
+Qed.
+
+Lemma po_in_events_l : forall (execArm : @Execution LabelArm LabelClassArm) x y,
+    well_formed_po execArm -> po execArm x y ->  events execArm x.
+Proof with eauto.
+    intros. unfold well_formed_po in *. destruct H as [H1 H2]. apply H1 in H0. destruct H0 as [H0 _]...
+Qed.
+
+Lemma po_in_events_r : forall (execArm : @Execution LabelArm LabelClassArm) x y,
+    well_formed_po execArm -> po execArm x y -> events execArm y.
+Proof with eauto.
+    intros. unfold well_formed_po in *. destruct H as [H1 H2]. apply H1 in H0. destruct H0 as [_ H0]...
+Qed.  
